Blaster/Command/Tactic.lean
@@ -34,56 +34,37 @@ def blasterTacticImp : Tactic := fun stx =>
    -- Parse options in any order
    let opts := stx[1].getArgs
    let sOpts ← parseSolveOptions opts default
-   let (goal, nbQuantifiers) ← revertHypotheses (← getMainGoal)
+   let goal ← revertHypotheses (← getMainGoal)
    let env := {(default : TranslateEnv) with optEnv.options.solverOptions := sOpts}
    let ((result, optExpr), _) ←
      withTheReader Core.Context (fun ctx => { ctx with maxHeartbeats := 0 }) $ do
        IO.setNumHeartbeats 0
-       Translate.main (← goal.getType >>= instantiateMVars') (logUndetermined := false) |>.run env
+       Translate.main (← goal.getType) (logUndetermined := false) |>.run env
    match result with
    | .Valid => goal.admit -- TODO: replace with proof reconstruction
    | .Falsified cex => throwTacticEx `blaster goal "Goal was falsified (see counterexample above)"
    | .Undetermined =>
         -- Replace the goal with the optimized expression
         let newGoal ← goal.replaceTargetDefEq optExpr
-        -- reintroduce reverted quantifiers
-        let currQuantifiers ← getFirstNbQuantifiers optExpr
-        let (_, newGoal') ← newGoal.introNP (max currQuantifiers nbQuantifiers)
-        replaceMainGoal [newGoal']
+        replaceMainGoal [newGoal]
 
   where
-    getFirstNbQuantifiers (e : Expr) : MetaM Nat := do
-      forallTelescope e fun fvars _ => do
-        let mut nb := 0
-        for v in fvars do
-          if !(← isProp (← v.fvarId!.getType)) then
-            nb := nb + 1
-        return nb
 
     @[always_inline, inline]
-    instantiateMVars' (e : Expr) : TacticM Expr :=
-     if e.hasMVar then instantiateMVars e else return e
-
-    @[always_inline, inline]
-    revertHypotheses (goal : MVarId) : TacticM (MVarId × Nat) :=
+    revertHypotheses (goal : MVarId) : TacticM MVarId :=
       goal.withContext $ do
         -- Get all hypotheses from the local context
         let lctx ← getLCtx
         let mut hyps := #[]
-        let mut nbQuantifiers := 0
         for decl in lctx do
           if decl.isImplementationDetail then continue
-          let declType ← instantiateMVars' decl.type
-          if !(← isProp declType) then
-            nbQuantifiers := nbQuantifiers + 1
-          hyps := hyps.push decl.fvarId
+          if ← isProp decl.type then
+            hyps := hyps.push decl.fvarId
         -- revert hyp from context
-        let goal' ←
-          hyps.foldrM
+        hyps.foldrM
           (fun h g => do
              let (_, g) ← g.revert #[h]
              return g) goal
-        return (goal', nbQuantifiers)
 
 
 end Blaster.Tactic
