Blaster/Optimize/Rewriting/OptimizeExists.lean
@@ -15,7 +15,7 @@ def coiExists (f : Expr) (args : Array Expr) : TranslateEnvT Expr := do
   if args.size != 2 then throwEnvError "coiExists: two arguments expected but got {reprStr args}"
   match args[1]! with
   | Expr.lam _n t e _bi =>
-      if (← (isSortOrInhabited t) <&&> (pure !(e.hasLooseBVar 0))) then return e
+      if (← (isSortOrInhabited t (existsQuantifier := true)) <&&> (pure !(e.hasLooseBVar 0))) then return e
       return mkAppN f args
   | _ => throwEnvError "coiExists: lambda expression expected but got {reprStr args[1]!}"
 
