Tests/FixedIssues.lean
@@ -27,6 +27,6 @@ import Tests.FixedIssues.Issue27
 import Tests.FixedIssues.Issue28
 import Tests.FixedIssues.Issue29
 import Tests.FixedIssues.Issue30
-
+import Tests.FixedIssues.Issue31
 import Tests.FixedIssues.Issue32
 import Tests.FixedIssues.Issue33
