Tests/FixedIssues/Issue20.lean
@@ -7,12 +7,28 @@ namespace Tests.Issue20
 -- Diagnosis : We need to generate extensionality assertion for each HOF function
 --             i.e., ∀ x, f x = g x → f = g
 
-theorem funextEq {α β : Type} (f g : α → β) : (f = g) = ∀ x, f x = g x := by
+theorem funextEq_poly {α β : Type} (f g : α → β) : (f = g) = ∀ x, f x = g x := by
       apply propext
       constructor
       { intro h ; simp only [h, implies_true] }
       { intro h ; apply funext h }
 
-#blaster [funextEq]
+#blaster [funextEq_poly]
+
+theorem funextEq_one_inst {β : Type} (f g : Nat → β) : (f = g) = ∀ x, f x = g x := by
+      apply propext
+      constructor
+      { intro h ; simp only [h, implies_true] }
+      { intro h ; apply funext h }
+
+#blaster [funextEq_one_inst]
+
+theorem funextEq_two_inst (f g : Nat → Int) : (f = g) = ∀ x, f x = g x := by
+      apply propext
+      constructor
+      { intro h ; simp only [h, implies_true] }
+      { intro h ; apply funext h }
+
+#blaster [funextEq_two_inst]
 
 end Tests.Issue20
