Tests/FixedIssues/Issue25.lean
@@ -5,19 +5,23 @@ open Lean Meta
 namespace Tests.Issue25
 
 -- Issue: translateType: unexpected sort type Lean.Expr.sort (Lean.Level.param `u_1)
--- Diagnosis : We need to normalize `sort (.params ..)` and `sort (.mvar ..)` to  `sort (.succ level.zero)`
---             during optimization phase.
+-- Diagnosis : We need to normalize `sort (.mvar m)` to `sort l`
+--             during optimization phase. It is expected that `m` must be assigned to `l`
+--             in the Lean4 environment. Otherwise we error.
+--             We also need to generate a distinct type universe at the smt level for each
+--             unique `·sort ..` expression.
 
 axiom hash : α → String
-axiom hash_collision_prop : ∀ (s1 s2 : α), hash s1 = hash s2 → s1 = s2
-axiom hash_size : ∀ (s : α), (hash s).length = 256
+
+axiom hash_collision_prop : ∀ (α : Type) (s1 s2 : α), hash s1 = hash s2 → s1 = s2
+axiom hash_size : ∀ (α : Type) (s : α), (hash s).length = 256
 
 -- check if we have a counterexample of length 256
 #blaster (gen-cex: 0) (solve-result: 1) [∀ (α : Type) (s : α), (hash s).length < 256]
 
 -- validate axiom
 #blaster (only-optimize: 1) [∀ (α : Type) (s : α), (hash s).length = 256]
--- Need to handle instantiation of polymorphic function
+-- Need to handle instantiation of polymorphic function as we need to instantiate the axioms
 -- #blaster [∀ (s : String), (hash s).length = 256]
 
 -- check if we are not wrongly applying axiom on another function
