Tests/FixedIssues/Issue31.lean
@@ -1,0 +1,124 @@
+import Lean
+import Blaster
+
+open Lean Meta
+namespace Tests.Issue31
+
+-- Issue: Unexpected Valid
+-- Diagnosis: We need to create a unique type universe at the SMT level for each sort.
+
+set_option warn.sorry false
+-- Valid expected
+theorem sort_unification_thm1 :
+  (∀ (β : Type) (x : β) (f : β → Nat), f x > 10) →
+  (∀ (α : Type) (x : α) (f : α → Nat), f x > 10) := by
+  intro h1 α x f
+  apply h1 α x f
+
+#blaster [sort_unification_thm1]
+
+-- Counterexample expected as β has Type u while α has Type 1
+theorem sort_unification_thm2 :
+  (∀ (x : β) (f : β → Nat), f x > 10) →
+  (∀ (α : Type) (x : α) (f : α → Nat), f x > 10) := by sorry
+   -- intro h1 α x f
+   -- apply h1 α x f can't apply h1
+
+#blaster (gen-cex: 0) (solve-result: 1) [sort_unification_thm2]
+
+-- Valid expected
+theorem sort_unification_thm3 :
+  (∀ (β : Type u) (x : β) (f : β → Nat), f x > 10) →
+  (∀ (α : Type u) (x : α) (f : α → Nat), f x > 10) := by
+   intro h1 α x f
+   apply h1 α x f
+
+#blaster [sort_unification_thm3]
+
+-- Counterexample expected as β has Type u + 1 while α has Type v + 1
+theorem sort_unification_thm4 :
+  (∀ (β : Type u) (x : β) (f : β → Nat), f x > 10) →
+  (∀ (α : Type v) (x : α) (f : α → Nat), f x > 10) := by sorry
+   -- intro h1 α x f
+   -- apply h1 α x f can't apply h1
+
+#blaster (gen-cex: 0) (solve-result: 1) [sort_unification_thm4]
+
+-- Valid expected
+theorem sort_unification_thm5 :
+  (∀ (β : Type u) (x : β) (f : β → Nat), f x > 10) →
+  (∀ (α : Type u) (x : α) (f : α → Nat), f x > 10) := by
+   intro h1 α x f
+   apply h1 α x f
+
+#blaster [sort_unification_thm5]
+
+-- Valid expected
+theorem sort_unification_thm6 :
+  (∀ (α : Type u) (β : Type v) (x : α) (f : α → β) (g : β → Nat), g (f x) > 10) →
+  (∀ (A : Type u) (B : Type v) (x : A) (m : A → B) (n : B → Nat), n (m x) > 10) := by
+  intro h1 α β x f g
+  apply h1 α β x f g
+
+#blaster [sort_unification_thm6]
+
+-- Counterexample expected as β has Type v + 1 while B has Type v + 2
+theorem sort_unification_thm7 :
+  (∀ (α : Type u) (β : Type v) (x : α) (f : α → β) (g : β → Nat), g (f x) > 10) →
+  (∀ (A : Type u) (B : Type (v + 1)) (x : A) (m : A → B) (n : B → Nat), n (m x) > 10) := by sorry
+  -- intro h1 α β x f g
+  -- apply h1 α β x f g -- can't apply h1
+
+#blaster (gen-cex: 0) (solve-result: 1) [sort_unification_thm7]
+
+-- Counterexample expected as β and α are within the same scope and
+-- therefore represent different types
+variable (B : Type u)
+theorem sort_unification_thm8 :
+  (∀ (x : B) (f : B → Nat), f x > 10) →
+  (∀ (α : Type u) (x : α) (f : α → Nat), f x > 10) := by sorry
+  -- intro h α x f
+  -- apply h x f -- can't apply h
+
+#blaster (gen-cex: 0) (solve-result: 1)  [sort_unification_thm8]
+
+
+theorem exists_must_match_forall :
+  ∀ (α : Type u), (∃ (β : Type u), α = β) := by
+  intro α
+  exact ⟨α, rfl⟩
+
+#blaster [exists_must_match_forall]
+
+theorem exist_nat_type : ∃ (α : Type), α = Nat := by exact ⟨Nat, rfl⟩
+
+#blaster [exist_nat_type]
+
+theorem exist_nat_type_with_instance: ∃ (a : Type) (_x : a), a = Nat := by exists Nat; exists 0
+#blaster [exist_nat_type_with_instance]
+
+-- Counterexample expect as there is no instance for Empty
+theorem exist_empty_type_with_instance : ∃ (a : Type) (x : a), a = Empty := by sorry
+  -- exists Empty;
+  -- can't provide an instance for x
+#blaster (gen-cex: 0) (solve-result: 1) [exist_empty_type_with_instance]
+
+theorem exist_type_with_instance : ∀ (b : Type), ∃ (a : Type) (_x : a), a = b := by sorry
+  -- intro b
+  -- exists b;
+  -- can't provide an instance for x
+#blaster (gen-cex: 0) (solve-result: 1) [exist_type_with_instance]
+
+theorem exist_list_nat_type : ∃ (a : Type), a = List Nat := by exists (List Nat)
+#blaster [exist_list_nat_type]
+
+theorem exist_list_nat_type_with_instance : ∃ (a : Type) (_x: a), a = List Nat := by exists (List Nat); exists []
+#blaster [exist_list_nat_type_with_instance]
+
+theorem exist_list_gen_type_with_instance : ∀ (b : Type), ∃ (a : Type) (_x: a), a = List b := by
+  intro b;
+  exists (List b); exists []
+
+#blaster [exist_list_gen_type_with_instance]
+
+end Tests.Issue31
